implemented SendServerParameters

hs/app/effect.hs
@@ -1,0 +1,108 @@
+{-# LANGUAGE ScopedTypeVariables #-}
+
+import qualified Data.ByteString as B
+import qualified Data.ByteString.Char8 as C
+import Network.Socket
+import qualified Network.Socket.ByteString as SB
+import Network.TLS
+import qualified Network.TLS.Internal as I
+import Crypto.Random
+import TLS
+
+main :: IO ()
+main = withSocketsDo $ do
+  sock <- socket AF_INET Stream 0
+  bind sock (SockAddrInet 8001 iNADDR_ANY)  
+  listen sock 2
+  (s,_) <- accept sock
+  core s (Left ()) RecvClientHello (unsafeCoerce 1)
+--  ehs <- recvHandshakes s
+  --SB.sendAll s $ C.pack "this is a dummy message"
+--  case ehs of
+    --Right hs -> print hs
+
+core sock x ef (r::Any) = do
+  case doHandshake_step x ef (unsafeCoerce r) of
+    Right res -> putStrLn "done"
+    Left (next, Nothing) -> core sock next RecvClientHello (unsafeCoerce 0)
+    Left (next, Just (ExistT e a)) ->
+      case e of
+        RecvClientHello ->
+          putStrLn "receive" >> recvClientHello sock >>= core sock next RecvClientHello . unsafeCoerce
+        GetRandomBytes -> do
+          putStrLn "getrandom"
+          v <- (getRandomBytes (unsafeCoerce a) :: IO B.ByteString)
+          putStrLn "getrandom finished"
+          core sock next GetRandomBytes (unsafeCoerce v)
+        SendPacket -> do
+          putStrLn "send"
+          bs <- encodePacket13 $ unsafeCoerce a
+          print (unsafeCoerce a :: I.Packet13)
+          putStrLn "\n"
+          case bs of
+            Right b ->
+              SB.sendAll sock b
+          core sock next SendPacket $ unsafeCoerce ()
+
+recvBytes :: Socket -> Int -> IO B.ByteString
+recvBytes sock n = B.concat <$> loop n
+  where loop 0 = return []
+        loop left = do
+          r <- (SB.recv sock left:: IO B.ByteString)
+          if B.null r
+            then return []
+            else (r:) <$> loop (left - B.length r)
+
+recvClientHello sock = do
+  ehss <- recvHandshakes sock
+  case ehss of
+    Right [I.ClientHello13 ver cRandom session cipherIDs exts] ->
+      return $ Build_ClientHelloMsg session exts cipherIDs
+
+recvHandshakes :: Socket -> IO (Either TLSError [I.Handshake13])
+recvHandshakes sock = do
+  erecord <- recvRecord sock
+  case erecord of
+    Left err -> return $ Left err
+    Right (I.Record ProtocolType_Handshake ver fragment) ->
+        return $ I.decodeHandshakes13 $ I.fragmentGetBytes fragment
+
+recvRecord :: Socket -> IO (Either TLSError (I.Record I.Plaintext))
+recvRecord sock = recvBytes sock 5 >>= recvLengthE . I.decodeHeader
+  where recvLengthE = either (return . Left) recvLength
+        recvLength header@(Header _ _ readlen)
+          | readlen > 16384 + 256 = return $ Left maximumSizeExceeded
+          | otherwise = do
+                bs <- recvBytes sock (fromIntegral readlen)
+                case I.runRecordM (I.decodeRecordM header bs) newRecordOptions I.newRecordState of
+                        Left err -> return $ Left err
+                        Right (a,_) -> return $ Right a
+
+newRecordOptions = I.RecordOptions { I.recordVersion = TLS13, I.recordTLS13 = True }
+
+maximumSizeExceeded :: TLSError
+maximumSizeExceeded = Error_Protocol ("record exceeding maximum size", True, RecordOverflow)
+
+
+encodePacket13 :: I.Packet13 -> IO (Either TLSError B.ByteString)
+encodePacket13 pkt = do
+    let pt = I.contentType pkt
+        mkRecord bs = I.Record pt TLS12 (I.fragmentPlaintext bs)
+        records = map mkRecord $ packetToFragments 16384 pkt
+    fmap B.concat <$> I.forEitherM records encodeRecord
+
+prepareRecord :: I.RecordM a -> IO (Either TLSError a)
+prepareRecord rm = case I.runRecordM rm newRecordOptions I.newRecordState of
+                        Left err -> return $ Left err
+                        Right (a,_) -> return $ Right a
+
+encodeRecord :: I.Record I.Plaintext -> IO (Either TLSError B.ByteString)
+encodeRecord = prepareRecord . I.encodeRecordM
+
+packetToFragments :: Int -> I.Packet13 -> [B.ByteString]
+packetToFragments len (I.Handshake13 hss)  =
+    I.getChunks len $ B.concat $ map I.encodeHandshake13 hss
+packetToFragments _   (I.Alert13 a)        = [I.encodeAlerts a]
+packetToFragments _   (I.AppData13 x)      = [x]
+packetToFragments _   I.ChangeCipherSpec13 = [I.encodeChangeCipherSpec]
+
