src/TLS.v
@@ -2,8 +2,8 @@ Require Import List.
 Require Import Inhabit Foldable ClConv.
 Import ListNotations.
 
-Definition byte := Ascii.ascii.
-Definition string := list byte.
+Parameter String : Set.
+Parameter ByteString : Set.
 
 Inductive Group := P256 | P384 | P521 | X25519.
 
@@ -27,137 +27,22 @@ Scheme Equality for Group.
 Scheme Equality for PskMode.
 Scheme Equality for SignatureScheme.
 
-(*
-Definition defaultCurvePreference :=
-  [X25519; CurveP256; CurveP384; CurveP521].
- *)
 
 Record KeyShare :=
   { KSgroup : Group;
-    KSdata : string
+    KSdata : ByteString
   }.
-
-Record PskIdentity :=
-  { PIlabel : list byte;
-    PIobfuscatedTicketAge : nat
-  }.
-
-Record Certificate :=
-  { Ccertificate : list (list byte);
-    CprivateKey : list byte;
-    COSPStable : list byte;
-    CSignedCertificateTimestamps : list (list byte);
-    CLeaf : list byte
-  }.
-
-Record SessionStateTLS13 :=
-  { STcipherSuite : nat;
-    STcreatedAt : nat;
-    STresumptionSecret : list byte;
-    certificate : Certificate
-  }.
-
-(*
-Record ServerHelloMsg :=
-  { (* SHlegacy_version : nat;*)
-    SHrandom : list byte;
-(*     SHlegacy_sessionID : list nat;*)
-    SHcipherSuite : nat;
-(*    SHlegacy_compressionMethod : nat; *)
-    SHsupportedVersion : nat;
-    SHserverShare : option KeyShare;
-    SHselectedCurve : option CurveID
-  }.
-*)
 
 Parameter ExtensionRaw : Set.
+Parameter Session : Set.
+Parameter CipherID : Set.
+
 Record ClientHelloMsg :=
   {
-    CHextension : list ExtensionRaw;
+    chSession : Session;
+    chExtension : list ExtensionRaw;
+    chCiphers : list CipherID
   }.
-
-(*
-  { (* CHlegacy_version_ : nat;*)
-    CHrandom : list byte;
-(*    CHlegacy_sessionID : list nat; *)
-    CHcipherSuites : list byte;
-(*    CHlegacy_compressionMethod : nat; *)
-    CHsupportedCurves : list CurveID;
-    CHkeyShares : list KeyShare;
-    CHpskModes : list nat;
-    CHpskIdentities : list PskIdentity;
-    CHserverName : String.string;
-    CHsupportedSignatureAlgorithms : list SignatureScheme
-  }.
-*)
-
-Record CipherSuiteTLS13 :=
-  { CSid : nat;
-    CSkeyLen : nat;
-  }.
-
-(*
-Record ServerHandshakeState :=
-  { SHSclientHello : ClientHelloMsg;
-    SHSserverHello : ServerHelloMsg
-  }.
-*)
-Parameter curve25519_scalarBaseMult : list byte -> list byte.
-Parameter curve25519_scalarMult : list byte -> list byte -> list byte.
-(*
-Parameter scalarMult : CurveID -> nat -> nat -> list byte -> list byte.
-Parameter scalarBaseMult : CurveID -> list byte -> nat * nat.
-Parameter elliptic_Marshal : CurveID -> nat * nat -> list byte.
-Parameter elliptic_Unmarshal : CurveID -> list byte -> nat * nat.
-Parameter paramSize : CurveID -> nat.
-Parameter nat_to_byte : nat -> byte.
-
-Parameter clientHelloMsg_marshal : ClientHelloMsg -> list byte.
-Parameter serverHelloMsg_marshal : ServerHelloMsg -> list byte.
-
-Parameter sessionStateTLS13_marshal : SessionStateTLS13 -> list byte.
-Parameter sessionStateTLS13_unmarshal : list byte -> SessionStateTLS13.
-
-Parameter VersionTLS13 : nat.
-Parameter helloRetryRequestRandom : list byte.
-
-Parameter decryptTicket : list byte -> list byte.
-
-Parameter signatureSchemesForCertificate :
-  nat -> Certificate -> list SignatureScheme.
-
-Definition typeMessageHash := (0,(1,(1,(1,(1,(1,(1,1))))))).
-
-Parameter hash : list byte -> list byte.
-*)
-(*
-Definition doHelloRetryRequest (ch : ClientHelloMsg)(sh : ServerHelloMsg)
-           (selectedCurve : CurveID) :=
-  let chHash := hash (clientHelloMsg_marshal ch) in
-  let helloRetryRequest :=
-      { SHrandom := helloRetryRequestRandom;
-        SHcipherSuite := sh.(SHcipherSuite);
-        SHsupportedVersion := sh.(SHsupportedVersion);
-        SHserverShare := None;
-        SHselectedCurve := selectedCurve }
-  in
-  let transcript :=
-      typeMessageHash :: x00 :: x00 :: nat_to_byte (length chHash)
-                      :: chHash ++ serverHelloMsg_marshal helloRetryRequest
-  in
-  
-  c <- writeRecord (serverHelloMsg_marshal helloRetryRequest);
-    sendDummyChangeCipherSpec;
-    msg <- readHandshake c;
-    let clientHello := msg.(ClientHelloMsg) in
-    match clientHello.(CHkeyShares) with
-    | [ks] =>
-      if not (CurveID_beq ks.(KSgroup) selectedCurve) then
-        Return (inr "Client sent invalid key share in second ClientHello")
-      else
-        (* ... *)
-        Return (inl clientHello)
-*)
 
 Ltac nth_of_tuple' p n flag :=
   lazymatch n with
@@ -188,17 +73,10 @@ Notation "p ._( n )" :=
   ltac:(nth_of_tuple p n)
          (at level 0, only parsing).
 
-(*
-Definition elliptic_GenerateKey (curve : CurveID) :=
-  private <- getRnd;
-    let public := scalarBaseMult curve private in
-    Return (private,public).
-*)
-
 Parameter ServerParams : Set.
 Parameter Context : Set.
 
-Parameter serverGroups : Context -> list Group.
+Parameter serverGroups : list Group.
 
 Fixpoint findKeyShare ks gs :=
   match gs with
@@ -215,19 +93,32 @@ Definition intersect (xs ys : list Group) :=
 
 Parameter extension_KeyShare : list ExtensionRaw -> option (list KeyShare).
 Parameter extension_NegotiatedGroups : list ExtensionRaw -> list Group.
+Parameter word32 : Set.
 
-Inductive eff_tls := recvClientHello | generateRND.
+Inductive PskIdentity := Build_PskIdentity : ByteString -> word32 -> PskIdentity.
+
+Inductive PreSharedKey :=
+| PreSharedKeyClientHello : list PskIdentity -> list ByteString -> PreSharedKey
+| PreSharedKeyServerHello : nat -> PreSharedKey.
+
+Parameter extension_PreSharedKey : list ExtensionRaw -> option PreSharedKey.
+Parameter Handshake13 : Set.
+Parameter Packet13 : Set.
+
+Inductive eff_tls := recvClientHello | getRandomBytes | sendPacket.
 
 Definition args_tls ef :=
   match ef with
-  | recvClientHello => Context
-  | generateKey => unit
+  | recvClientHello => unit
+  | getRandomBytes => nat
+  | sendPacket => Packet13
   end.
 
 Definition rets_tls ef :=
   match ef with
   | recvClientHello => ClientHelloMsg
-  | generateKey => string
+  | getRandomBytes => ByteString
+  | sendPacket => unit
   end.
 
 Definition lift_tls A B(e : eff_tls)(a : rets_tls e -> A + option B) e0
@@ -242,10 +133,16 @@ Definition lift_tls A B(e : eff_tls)(a : rets_tls e -> A + option B) e0
       | recvClientHello => a0
       | _ => fun _ => inr None
       end
-  | generateRND =>
-    fun a0 : rets_tls generateRND -> A + option B =>
+  | getRandomBytes =>
+    fun a0 : rets_tls getRandomBytes -> A + option B =>
       match e0 as e1 return (rets_tls e1 -> A + option B) with
-      | generateRND => a0
+      | getRandomBytes => a0
+      | _ => fun _ => inr None
+      end
+  | sendPacket =>
+    fun a0 : rets_tls sendPacket -> A + option B =>
+      match e0 as e1 return (rets_tls e1 -> A + option B) with
+      | sendPacket => a0
       | _ => fun _ => inr None
       end
   end a.
@@ -259,34 +156,173 @@ Notation "ch <-recvClientHello ctx ; p" :=
   (@Eff eff_tls args_tls rets_tls _ recvClientHello ctx (fun ch => p))
     (at level 100, right associativity).
 
-Definition pickKeyShare
-           (ctx : Context) :=
-  ch <-recvClientHello ctx;
-    match extension_KeyShare ch.(CHextension) with
+Notation "b <-getRandomBytes n ; p" :=
+  (@Eff eff_tls args_tls rets_tls _ getRandomBytes n (fun b => p))
+    (at level 100, right associativity).
+
+Notation "'sendPkt' b ; p" :=
+  (@Eff eff_tls args_tls rets_tls _ sendPacket b (fun _ => p))
+    (at level 200, right associativity).
+
+Definition option_beq {A} (A_beq : A -> A -> bool) o1 o2 :=
+  match o1, o2 with
+  | None, None => true
+  | Some a1, Some a2 => A_beq a1 a2
+  | _,_ => false
+  end.
+
+Parameter Hash : Set.
+Parameter HostName : Set.
+Parameter ctxGetClientSNI : Context -> option HostName.
+Parameter ctxGetNegotiatedProtocol : Context -> option ByteString.
+Parameter Cipher : Set.
+Parameter CipherID_beq : CipherID -> CipherID -> bool.
+Parameter SessionData : Set.
+Parameter sessionCipher : SessionData -> CipherID.
+Parameter cipherID : Cipher -> CipherID.
+Parameter serverSupportedCiphers : ServerParams -> list Cipher.
+Parameter Hash_beq : Hash -> Hash -> bool.
+Parameter cipherHash : Cipher -> Hash.
+Parameter Version : Set.
+Parameter Version_beq : Version -> Version -> bool.
+Parameter sessionVersion : SessionData -> Version.
+Parameter ByteString_beq : ByteString -> ByteString -> bool.
+Parameter sessionALPN : SessionData -> option ByteString.
+
+Open Scope bool_scope.
+
+Definition checkSessionEquality ctx sparams chosenVersion usedCipher sdata :=
+  let msni := ctxGetClientSNI ctx in
+  let malpn := ctxGetNegotiatedProtocol ctx in
+  let isSameCipher := CipherID_beq (sessionCipher sdata) (cipherID usedCipher) in
+  let ciphers := serverSupportedCiphers sparams in
+  let isSameKDF :=
+      match find (fun c => CipherID_beq (cipherID c) (sessionCipher sdata)) ciphers with
+      | Some c => Hash_beq (cipherHash c) (cipherHash usedCipher)
+      | Nothing => false
+      end
+  in
+  let isSameVersion := Version_beq chosenVersion (sessionVersion sdata) in
+  let isSameALPN := option_beq ByteString_beq (sessionALPN sdata) malpn in
+  let is0RTTvalid := isSameVersion && isSameCipher && isSameALPN in
+  (isSameKDF, is0RTTvalid).
+
+Parameter PskKexMode : Set.
+Parameter PSK_DHE_KE : PskKexMode.
+Parameter extension_PskKeyExchangeModes : list ExtensionRaw -> option (list PskKexMode).
+Parameter PskKexMode_eq_dec : forall x y : PskKexMode, {x=y}+{x<>y}.
+Parameter zero : ByteString.
+Parameter Blength : ByteString -> nat.
+Parameter SessionManager : Set.
+Parameter serverSharedSessionManager : ServerParams -> SessionManager.
+Parameter sessionResume : SessionManager -> ByteString -> option SessionData.
+Parameter sessionResumeOnlyOnce : SessionManager -> ByteString -> option SessionData.
+Parameter sessionSecret : SessionData -> ByteString.
+Definition sum_nat xs := fold_left Nat.add xs 0.
+
+Definition choosePSK (rtt0:bool) ctx sparams chosenVersion usedCipher exts :=
+  match extension_PreSharedKey exts with
+  | Some (PreSharedKeyClientHello (Build_PskIdentity sessionId obfAge::_) (bnd::_ as bnds)) =>
+    match extension_PskKeyExchangeModes exts with
+    | None => (zero, None, false)
+    | Some dhModes =>
+      if in_dec PskKexMode_eq_dec PSK_DHE_KE dhModes then
+        let len := (sum_nat (map (fun x => Blength x + 1) bnds) + 2)%nat in
+        let mgr := serverSharedSessionManager sparams in
+        let msdata :=
+            if rtt0 then sessionResumeOnlyOnce mgr sessionId
+            else sessionResume mgr sessionId
+        in
+          match msdata with
+          | Some sdata =>
+            let psk := sessionSecret sdata in
+            let validity := checkSessionEquality ctx sparams chosenVersion usedCipher sdata in
+            if (fst validity) then
+              (psk, Some (bnd,0,len), snd validity)
+            else
+              (zero, None, false)
+          | Nothing => (zero, None, false)
+          end
+      else
+        (zero, None, false)
+    end
+  | _ => (zero, None, false)
+  end.
+
+Parameter extensionEncode_KeyShare : KeyShare -> ByteString.
+Parameter extensionEncode_SupportedVersions : Version -> ByteString.
+Parameter TLS13 : Version.
+Parameter extensionRaw_KeyShare : ByteString -> ExtensionRaw.
+Parameter extensionRaw_SupportedVersions : ByteString -> ExtensionRaw.
+Parameter handshake13 : list Handshake13 -> Packet13.
+Parameter serverHello13 : ByteString -> Session -> CipherID -> list ExtensionRaw -> Handshake13.
+
+Definition doHandshake :=
+  ch <-recvClientHello tt;
+    let opt := extension_KeyShare ch.(chExtension) in
+    match opt with
     | None => Return None
     | Some keyShares =>
-      match findKeyShare keyShares (serverGroups ctx) with
+      let oks := findKeyShare keyShares serverGroups in
+      match oks with
+      | None => Return None
+      | Some keyShare =>
+        (* sendServerHello *)
+        let serverKeyShare := extensionEncode_KeyShare keyShare in
+        let selectedVersion := extensionEncode_SupportedVersions TLS13 in
+        let extensions' := [ extensionRaw_KeyShare serverKeyShare;
+                             extensionRaw_SupportedVersions selectedVersion ]
+        in
+        srand <-getRandomBytes 32;
+          match hd_error (chCiphers ch) with
+          | None => Return None
+          | Some cipher =>
+            srand <-getRandomBytes 32;
+            sendPkt (handshake13 [serverHello13 srand (chSession ch) cipher extensions']);
+              Return (Some tt)
+          end
+      end
+    end.
+
+Definition doHandshake_derive :
+  { state & { step &
+                { init | @equiv _ _ _ _ state step init doHandshake }}}.
+Proof.
+  do 3 eexists.
+  unfold doHandshake.
+  derive' tt.
+Defined.
+
+Definition doHandshake_step := Eval cbv [projT1 projT2 doHandshake doHandshake_derive] in (projT1 (projT2 doHandshake_derive)).
+
+Definition pickKeyShare :=
+  ch <-recvClientHello tt;
+    match extension_KeyShare ch.(chExtension) with
+    | None => Return None
+    | Some keyShares =>
+      match findKeyShare keyShares (serverGroups) with
       | None =>
         (* helloRetryRequest *)
-        let clientGroups := extension_NegotiatedGroups ch.(CHextension) in
-        let possibleGroups := intersect (serverGroups ctx) clientGroups in
+        let clientGroups := extension_NegotiatedGroups ch.(chExtension) in
+        let possibleGroups := intersect (serverGroups) clientGroups in
         match hd_error possibleGroups with
         | None => Return None
         | Some g => 
-          ch' <-recvClientHello ctx;
-            match extension_KeyShare ch'.(CHextension) with
+          ch' <-recvClientHello tt;
+            match extension_KeyShare ch'.(chExtension) with
             | None => Return None
             | Some keyShares =>
-              match findKeyShare keyShares (serverGroups ctx) with
+              match findKeyShare keyShares (serverGroups ) with
               | None => Return None
               | Some keyShare => Return (Some (ch', keyShare))
               end
             end
         end
+        (* helloRetryRequest end *)
       | Some keyShare => Return (Some (ch, keyShare))
       end
     end.
-
+(*
 Definition pickKeyShare_derive :
   { state & { step & forall ctx,
                 { init | @equiv _ _ _ _ state step init (pickKeyShare ctx) }}}.
@@ -297,181 +333,51 @@ Proof.
 Defined.
 
 Definition pickKeyShare_step := Eval cbv [projT1 projT2 pickKeyShare pickKeyShare_derive] in (fun ctx => projT1 (projT2 pickKeyShare_derive) ctx).
+*)
+
 
 Extract Inductive unit => "()" [ "()" ].
 Extract Inductive list => "([])" ["[]" "(:)"].
+Extract Inductive nat => "Int" ["0" "(Prelude.+) 1"] "(\fO fS n -> if n==0 then fO () else fS (n Prelude.- 1))".
 Extract Inductive bool => "GHC.Base.Bool" ["GHC.Base.True" "GHC.Base.False"].
 Extract Inductive sumbool => "GHC.Base.Bool" ["GHC.Base.True" "GHC.Base.False"].
 Extract Inductive prod => "(,)"  [ "(,)" ].
 Extract Inductive sum => "Prelude.Either" ["Prelude.Left" "Prelude.Right"].
 Extract Inductive option => "GHC.Base.Maybe" ["GHC.Base.Just" "GHC.Base.Nothing"].
 Extract Inductive Group => "T.Group" ["T.P256" "T.P384" "T.P521" "T.X25519"].
-Extract Constant Group_eq_dec => "(==)".
-Extract Constant Group_beq => "(==)".
+Extract Inductive KeyShare => "I.KeyShareEntry" ["I.KeyShareEntry"].
+Extract Constant Group_eq_dec => "(GHC.Base.==)".
+Extract Constant Group_beq => "(GHC.Base.==)".
 Extract Constant Context => "T.Context".
 Extract Constant ExtensionRaw => "I.ExtensionRaw".
-Extract Constant string => "B.ByteString".
+Extract Constant Session => "I.Session".
+Extract Constant CipherID => "T.CipherID".
+Extract Constant Handshake13 => "I.Handshake13".
+Extract Constant Packet13 => "I.Packet13".
+Extract Constant ByteString => "B.ByteString".
+Extract Constant extensionEncode_KeyShare => "(\ks -> I.extensionEncode (I.KeyShareServerHello ks))".
+Extract Constant extensionEncode_SupportedVersions =>
+"(\v -> I.extensionEncode (I.SupportedVersionsServerHello v))".
+Extract Constant Version => "T.Version".
+Extract Constant TLS13 => "T.TLS13".
+Extract Constant extensionRaw_KeyShare => "I.ExtensionRaw I.extensionID_KeyShare".
+Extract Constant extensionRaw_SupportedVersions =>
+"I.ExtensionRaw I.extensionID_SupportedVersions".
+Extract Constant handshake13 => "I.Handshake13".
+Extract Constant serverHello13 => "(\b -> I.ServerHello13 (I.ServerRandom {I.unServerRandom = b}))".
+
+Extract Constant extension_KeyShare =>
+"(\exts -> case Helper.extensionLookup I.extensionID_KeyShare exts GHC.Base.>>= I.extensionDecode I.MsgTClientHello of { GHC.Base.Just (I.KeyShareClientHello kses) -> GHC.Base.return kses})".
+Extract Constant serverGroups => "Helper.serverGroups".
+
+(*
 Extract Constant extension_KeyShare => "Helper.extension_KeyShare".
 Extract Constant extension_NegotiatedGroups => "Helper.extension_NegotiatedGroups".
 Extract Constant serverGroups => "Helper.serverGroups".
 Extract Inductive KeyShare => "Helper.KeyShare" ["Helper.Build_KeyShare"].
+ *)
 
 Require Extraction.
 Extraction Language Haskell.
 
-Extraction "TLS.hs" pickKeyShare_step.
-
-(*
-srand <- getRnd;
-          protoExt <<- applicationProtocol ctx exts sparams
-                   (psk,binderInfo,is0RTTvalid) <<- choosePSK;
-          earlyKey <- calculateEarlySecret ctx choice (inl psk) true;
-          let earlySecret := pairBase earlyKey in
-                let clientEarlySecret := pairClient earlyKey in
-                
-    end
-  end
-*)
-
-Definition processClientHello (ch : ClientHelloMsg) :=
-  random <- getRnd;
-    let ks :=
-        list_rec_nondep
-          (fun opt =>
-             match opt with
-             | Some group =>
-               Some (doHelloRetryRequest group)
-             | None => None
-             end)
-          (fun preferredGroup restCurves recPref opt =>
-             list_rec_nondep
-               (match opt with
-                | Some group => recPref opt
-                | None =>
-                  if in_dec CurveID_eq_dec
-                            preferredGroup ch.(CHsupportedCurves) then
-                    recPref (Some preferredGroup)
-                  else
-                    recPref None
-                end)
-               (fun ks keyShares' rec =>
-                  if CurveID_beq ks.(KSgroup) preferredGroup then
-                    Some ks
-                  else
-                    rec)
-               ch.(CHkeyShares))
-          defaultCurvePreference
-          None
-    in
-    match ks with
-    | Some clientKeyShare =>
-      keys <<- (if CurveID_beq clientKeyShare.(KSgroup) X25519 then
-                  private <- getRnd;
-                    Return (curve25519_scalarBaseMult private,
-                     curve25519_scalarMult private clientKeyShare.(KSdata))
-                else
-                  let curveID := clientKeyShare.(KSgroup) in
-                  keys' <<- elliptic_GenerateKey curveID;
-                    Return
-                      (elliptic_Marshal curveID (snd keys'),
-                       let (x,y) :=
-                           elliptic_Unmarshal curveID clientKeyShare.(KSdata)
-                       in
-                       scalarMult curveID x y (fst keys'))
-               );
-      let share :=
-          {| KSgroup := clientKeyShare.(KSgroup);
-             KSdata := keys._(0) |}
-      in
-      Return (Some ({| SHrandom := random;
-                      SHcipherSuite := 0;
-                      SHsupportedVersion := VersionTLS13;
-                      SHserverShare := Some share;
-                      SHselectedCurve := Some share.(KSgroup) |},
-                   keys._(1)))
-    | None =>
-      Return None
-        (*(inr "No ECDHE curve supported by both client and server")*)
-    end.
-
-Definition processClientHello_derive :
-  { state & { step & forall ch,
-                { init | @equiv _ _ _ _ state step init (processClientHello ch) }}}.
-Proof.
-  do 3 eexists.
-  unfold processClientHello.
-  derive' (tt,ch).
-Defined.
-
-Eval cbv [projT1 projT2 processClientHello processClientHello_derive] in (fun ch => projT1 (projT2 processClientHello_derive) ch).
-
-Parameter getCertificate : String.string -> Map Certificate -> list Certificate -> option Certificate.
-
-(*
-Definition getCertificate
-           (serverName : Stirng.string)
-           (nameToCertificate : Map Certificate)
-           (certificates : list Certificate) :=
-  (* if c.GetCertificate != nil ... *)
-  match certificates with
-  | [] => None
-  | cerf::[] => Some cerf
-  | cerf::_ =>
-    let name := toLower serverName in
-    match bsearch name nameToCertificate with
-    | Some cerf' => Some cerf'
-    | None =>
- *)
-
-Definition pickCertificate
-           (clientHello : ClientHelloMsg)
-           (serverHello : ServerHelloMsg)
-           (usingPSK : bool)
-           (hs : ServerHandshakeState)
-           (nameToCertificate : Map Certificate)
-           (certificates : list Certificate) :=
-  if usingPSK then
-    None
-  else
-    match getCertificate clientHello.(CHserverName) nameToCertificate certificates with
-    | None => None
-    | Some certificate =>
-      let supportedAlgs :=
-          signatureSchemesForCertificate hs.(SHSserverHello).(SHsupportedVersion) certificate
-      in
-      list_rec_nondep
-        None
-        (fun preferredAlg rest aux =>
-           if in_dec SignatureScheme_eq_dec preferredAlg supportedAlgs then
-             Some preferredAlg
-           else
-             aux)
-        clientHello.(CHsupportedSignatureAlgorithms)
-    end.
-
-
-Definition checkForResumption (ch : ClientHelloMsg) suite :=
-  if in_dec PskMode_eq_dec PskModeDHE ch.(CHpskModes) then
-    list_rec_nondep
-      (Return None)
-      (fun identity rec =>
-         let plaintext := decryptTicket identity.(label) in
-         let sessionState := sessionStateTLS13_unmarshal plaintext in
-         let pskSuite := cipherSuiteTLS13ByID sessionState.(cipherSuite) in
-         if pskSuite.(hash)!= suite.(hash) then
-           rec
-         else
-           let sessionHasClientCerts :=
-               notb (Nat.eqb (sessionState.(certificate).(Certificate)) 0)
-           in
-           let needClientCerts :=
-               requiresClientCert c.(config).(ClientAuth)
-           in
-           if (needClientCerts && notb sessionHasClientCerts)
-              || (sessionHasClientCerts && c.(config).(ClientAuth) == NoClientCert) then
-             rec
-           else
-             Return (Some (extract suite))
-      )
-      ch.(CHpskIdentities)
-  else Return None.
+Extraction "TLS.hs" doHandshake_step.
